Adding support for pattern-matching on constructors of arbitrary arity

Ast.v
@@ -1,6 +1,6 @@
 Require Template.All.
 
-Require Import Template.Ast.
+Require Import Template.Ast Template.AstUtils.
 Require Import Template.Typing.
 Require Import String List.
 
@@ -11,8 +11,6 @@ Open Scope string_scope.
 Definition name := string.
 Definition inductive := string.
 
-Definition rName (nm : string) : Ast.aname := mkBindAnn (nNamed nm) Relevant.
-Definition rAnon : Ast.aname := mkBindAnn nAnon Relevant.
 
 Inductive type : Set :=
 | tyInd : inductive -> type
@@ -30,7 +28,12 @@ Definition stupid_case (b : bool) : nat :=
   | false => 0
   end.
 
-SearchPattern (bool -> bool).
+Definition stupid_case' (b : bool * bool) : nat :=
+  match b with
+  | (true, _) => 1
+  | (false, _) => 0
+  end.
+
 
 Definition is_zero (n : nat) :=
   match n with
@@ -39,9 +42,12 @@ Definition is_zero (n : nat) :=
   end.
 
 Quote Recursively Definition q_stupid_fix := stupid_fix.
-Definition Σ := (fst q_stupid_fix).
+
+Definition Σ := Eval compute in (fst q_stupid_fix).
 (* Eval compute in type_of_constructor Σ ((mkInd "Coq.Init.Datatypes.nat" 0),1) [] [] *)
 Quote Definition q_stupid_case := Eval compute in stupid_case.
+(* Nested patters are transformed into the nested "case" expressions *)
+Quote Definition q_stupid_case' := Eval compute in stupid_case'.
 Quote Definition q_is_zero := Eval compute in is_zero.
 Make Definition is_zero' := Eval compute in q_is_zero.
 Quote Definition q_plus := Eval compute in plus.
@@ -50,8 +56,7 @@ Quote Definition q_app := Eval compute in app.
 Definition ex_let n := let q := 1 in q + n.
 Quote Definition q_let := (fun n => let q := 1 in q + n).
 
-Inductive pat :=
-| pConstr : name -> list name -> pat.
+Record pat := pConstr {pName : name; pVars : list name}.
 
 Inductive expr : Set :=
 | eRel       : nat -> expr
@@ -59,15 +64,23 @@ Inductive expr : Set :=
 | eLambda    : name -> type -> expr -> expr
 | eLetIn     : name -> expr -> type -> expr -> expr
 | eApp       : expr -> expr -> expr
-| eConstruct : inductive -> nat -> expr
+| eConstr    : inductive -> name -> expr
 | eConst     : name -> expr
 | eCase      : (inductive * nat) (* # of parameters *) -> type
                -> expr (* discriminee *) -> list (pat * expr) (* branches *) -> expr
-(* | eProj      : projection -> expr -> expr *)
 | eFix       : name -> type -> expr -> expr.
-(* | eCoFix     : mfixpoint expr -> nat -> expr. *)
 
-(* eq_string *)
+Definition constr := (name * list type)%type.
+
+(* Could be extended to handle declaration of costanst, e.g. function definitions *)
+Inductive global_dec :=
+| gdInd : name -> list constr -> global_dec.
+
+Definition global_env := list global_dec.
+
+(* Associates names of types and constants of our langauge to the corresponding names in Coq *)
+Definition translation_table := list (name * name).
+
 
 Fixpoint lookup {A} (l : list (string * A)) key : option A :=
   match l with
@@ -75,32 +88,67 @@ Fixpoint lookup {A} (l : list (string * A)) key : option A :=
   | (key', v) :: xs => if eq_string key' key then Some v else lookup xs key
   end.
 
+Fixpoint lookup_global ( Σ : global_env) key : option global_dec :=
+  match Σ with
+  | [] => None
+  | gdInd key' v :: xs => if eq_string key' key then Some (gdInd key' v) else lookup_global xs key
+  end.
+
+Definition find_i {A : Type} (f : A -> bool) (l : list A) :=
+let fix find (i : nat) (l : list A) : option (nat * A) :=
+  match l with
+  | [] => None
+  | x :: tl => if f x then Some (i,x) else find (1+i) tl
+  end in
+find 0 l.
+
+(* Resolves the constructor name to a corresponding position in the list of costructors along
+   with the constructor info *)
+Definition resolve_constr (Σ : global_env) (ind_name constr_name : ident)
+  : option (nat * (string * list type)) :=
+  match (lookup_global Σ ind_name) with
+  | Some (gdInd n cs) => find_i (fun x => proj1_sig (Sumbool.bool_of_sumbool (string_dec (fst x) constr_name))) cs
+  | None => None
+  end.
+
+
 Definition from_option {A : Type} ( o : option A) (default : A) :=
   match o with
   | None => default
   | Some v => v
   end.
 
+Definition bump_indices (l : list (name * nat)) (n : nat) :=
+  map (fun '(x,y) => (x, n+y)) l.
+
+(* For a list of vars returns a list of pairs (var,number)
+where the number is a position of the var counted from the end of the list.
+ E.g. number_vars ["x"; "y"; "z"] = [("x", 2); ("y", 1); ("z", 0)] *)
+Definition number_vars (ns : list name) : list (name * nat) :=
+  combine ns (rev (seq 0 (length ns))).
+
+Example number_vars_xyz : number_vars ["x"; "y"; "z"] = [("x", 2); ("y", 1); ("z", 0)].
+Proof. reflexivity. Qed.
+
 Fixpoint indexify (l : list (name * nat)) (e : expr) : expr :=
   match e with
   | eRel i => eRel i
   | eVar nm =>
     match (lookup l nm) with
-    | None => eVar ("not a closed term") (* a hack to make the function total *)
+    | None => (* FIXME: a hack to make the function total *)
+      eVar ("not a closed term")
     | Some v => eRel v
     end
   | eLambda nm ty b =>
-    let bump_list := map (fun '(x,y) => (x, 1+y)) l in
-    eLambda nm ty (indexify ((nm,0 ):: bump_list) b)
+    eLambda nm ty (indexify ((nm,0 ):: bump_indices l 1) b)
   | eLetIn nm e1 ty e2 =>
-    let bump_list := map (fun '(x,y) => (x, 1+y)) l in
-    eLetIn nm e1 ty (indexify ((nm, 0) :: bump_list) e2)
+    eLetIn nm e1 ty (indexify ((nm, 0) :: bump_indices l 1) e2)
   | eApp e1 e2 => eApp (indexify l e1) (indexify l e2)
-  | eConstruct t i as e => e
+  | eConstr t i as e => e
   | eConst nm as e => e
   | eCase nm_i ty e bs =>
-    (* bracnhes are not handled properly yet; this only works for pattrens not binding any vars *)
-    eCase nm_i ty (indexify l e) bs
+    eCase nm_i ty (indexify l e)
+          (map (fun p => (fst p, indexify (number_vars (fst p).(pVars) ++ bump_indices l (length (fst p).(pVars))) (snd p))) bs)
   | eFix nm ty b =>
     let bump_list := map (fun '(x,y) => (x, 1+y)) l in
     eFix nm ty (indexify ((nm, 0) :: bump_list) b)
@@ -109,43 +157,60 @@ Fixpoint indexify (l : list (name * nat)) (e : expr) : expr :=
 Fixpoint type_to_term (ty : type) : term :=
   match ty with
   | tyInd i => tInd (mkInd i 0) []
-  | tyArr t1 t2 => tProd rAnon (type_to_term t1) (type_to_term t2)
+  | tyArr t1 t2 => tProd nAnon (type_to_term t1) (type_to_term t2)
   end.
 
-SearchPattern (list _ -> list _ -> list _).
 
-Definition numbered {A : Type} (l : list A) := combine (seq 0 (length l)) l.
+Fixpoint pat_to_lam (tys : list (name * type)) (body : term) : term :=
+  match tys with
+    [] => body
+  | (n,ty) :: tys' => tLambda (nNamed n) (type_to_term ty) (pat_to_lam tys' body)
+  end.
 
-Fixpoint expr_to_term (e : expr) : Ast.term :=
+SearchPattern (list _ -> list _ -> list (_ * _)).
+
+(* Resolves a pattern by looking up in the global environment
+   and returnes a list of pairs mapping pattern variable
+names to the types of the constructor arguments *)
+Definition resolve_pat_arity (Σ : global_env) (ind_name : name) (p : pat) :=
+  (* FIXME: in lookup failed we return a dummy value [(0,("",[]))]
+     to make the function total *)
+  combine p.(pVars)
+  (snd (snd (from_option (resolve_constr Σ ind_name p.(pName)) (0,("",[]))))).
+
+Definition expr_to_term (Σ : global_env) : expr -> Ast.term :=
+  fix expr_to_term e :=
   match e with
   | eRel i => tRel i
   | eVar nm => tVar nm
-  | eLambda nm ty b => tLambda (mkBindAnn (nNamed nm) Relevant) (type_to_term ty) (expr_to_term b)
-  | eLetIn nm e1 ty e2 => tLetIn (rName nm) (expr_to_term e1) (type_to_term ty) (expr_to_term e2)
+  | eLambda nm ty b => tLambda (nNamed nm) (type_to_term ty) (expr_to_term b)
+  | eLetIn nm e1 ty e2 => tLetIn (nNamed nm) (expr_to_term e1) (type_to_term ty) (expr_to_term e2)
   | eApp e1 e2 => tApp (expr_to_term e1) [expr_to_term e2]
-  | eConstruct t i => tConstruct (mkInd t 0) i []
+  | eConstr t i => match (resolve_constr Σ t i) with
+                     | Some c => tConstruct (mkInd t 0) (fst c) []
+                     (* FIXME: a hack to make the function total *)
+                     | None => tVar ("No declaration found: " ++ t)
+                     end
   | eConst nm => tConst nm []
   | eCase nm_i ty e bs =>
-    (* this interpretation is not complete, it ignores patterns and
-       only works for constructors without parameters. Also, patterns must be in the same
-     order as constructors in the definition *)
+    (* this interpretation is not complete, no translation for polymorphic types.
+       Patterns must be in the same order as constructors in the definition *)
     let (nm,i) := nm_i in
-    let typeInfo := tLambda rAnon (tInd (mkInd nm 0) []) (type_to_term ty) in
-    tCase (mkInd nm 0, i) typeInfo None (expr_to_term e)
-          (List.map (fun x => (0, expr_to_term (snd x))) bs)
-  | eFix nm ty b => tFix [(mkdef _ (rName nm) (type_to_term ty) (expr_to_term b) 0)] 0
+    let typeInfo := tLambda nAnon (tInd (mkInd nm 0) []) (type_to_term ty) in
+    let tys n := resolve_pat_arity Σ nm (fst n) in
+    let branches :=
+        List.map (fun x => (length (fst x).(pVars), pat_to_lam (tys x) (expr_to_term (snd x)))) bs in
+    tCase (mkInd nm 0, i) typeInfo (expr_to_term e) branches
+  | eFix nm ty b => tFix [(mkdef _ (nNamed nm) (type_to_term ty) (expr_to_term b) 0)] 0
   end.
 
 Module BaseTypes.
   Definition Nat_name := "Coq.Init.Datatypes.nat".
   Definition Nat := tyInd Nat_name.
-  Definition Z := eConstruct Nat_name 0.
-  Definition Suc := eConstruct Nat_name 1.
-
   Definition Bool_name := "Coq.Init.Datatypes.bool".
   Definition Bool := tyInd Bool_name.
-  (* Definition true := eConstruct Bool_name 0. *)
-  (* Definition false := eConstruct Bool_name 1. *)
+  (* Definition true := eConstr Bool_name 0. *)
+  (* Definition false := eConstr Bool_name 1. *)
 End BaseTypes.
 
 Import BaseTypes.
@@ -154,8 +219,8 @@ Declare Custom Entry expr.
 Declare Custom Entry pat.
 
 Notation "[| e |]" := e (e custom expr at level 2).
-Notation "x" := (eVar x) (in custom expr at level 0, x constr at level 4).
 Notation "^ i " := (eRel i) (in custom expr at level 3, i constr at level 4).
+Notation "x" := (eVar x) (in custom expr at level 0, x constr at level 4).
 Notation "\ x : ty -> b" := (eLambda x ty b)
                               (in custom expr at level 1,
                                   ty constr at level 4,
@@ -165,6 +230,10 @@ Notation "'let' x : ty := e1 'in' e2" := (eLetIn x e1 ty e2)
                                                ty constr at level 4,
                                                x constr at level 4).
 
+(* Notation "C x .. y" := (pConstr C (cons x .. (cons y nil) .. )) *)
+(*                          (in custom pat at level 1, *)
+(*                              x constr at level 4, *)
+(*                              y constr at level 4). *)
 
 (* Could not make recursive notation work, so below there are several variants
    of [case] for different number of cases *)
@@ -176,11 +245,6 @@ Notation "'let' x : ty := e1 'in' e2" := (eLetIn x e1 ty e2)
 (*         bn custom expr at level 4, *)
 (*         ty constr at level 4). *)
 
-Notation "'case' x : ty 'of' p1 -> b1 " :=
-  (eCase (ty,0) (tyInd "") x [(p1,b1)])
-    (in custom expr at level 1,
-        b1 custom expr at level 4,
-        ty constr at level 4).
 
 Notation "'case' x : ty1 'return' ty2 'of' | p1 -> b1 | pn -> bn" :=
   (eCase (ty1,0) ty2 x [(p1,b1);(pn,bn)])
@@ -192,39 +256,63 @@ Notation "'case' x : ty1 'return' ty2 'of' | p1 -> b1 | pn -> bn" :=
         ty1 constr at level 4,
         ty2 constr at level 4).
 
-Notation "'case' x : ty 'of' b1 | b2 | bn" :=
-  (eCase (ty,0) (tyInd "") x [b1;b2;bn])
+Notation "'case' x : ty1 'return' ty2 'of' p1 -> b1 " :=
+  (eCase (ty1,0) ty2 x [(p1,b1)])
     (in custom expr at level 1,
+        p1 custom pat at level 4,
         b1 custom expr at level 4,
-        b2 custom expr at level 4,
-        bn custom expr at level 4,
-        ty constr at level 4).
+        ty1 constr at level 4,
+        ty2 constr at level 4).
 
-Notation "'case' x : ty 'of' b1 | b2 | b3 | bn" :=
-  (eCase (ty,0) (tyInd "") x [b1;b2;b3;bn])
-    (in custom expr at level 1,
-        b1 custom expr at level 4,
-        b2 custom expr at level 4,
-        b3 custom expr at level 4,
-        bn custom expr at level 4,
-        ty constr at level 4).
+
+(* Notation "'case' x : ty 'of' b1 | b2 | bn" := *)
+(*   (eCase (ty,0) (tyInd "") x [b1;b2;bn]) *)
+(*     (in custom expr at level 1, *)
+(*         b1 custom expr at level 4, *)
+(*         b2 custom expr at level 4, *)
+(*         bn custom expr at level 4, *)
+(*         ty constr at level 4). *)
+
+(* Notation "'case' x : ty 'of' b1 | b2 | b3 | bn" := *)
+(*   (eCase (ty,0) (tyInd "") x [b1;b2;b3;bn]) *)
+(*     (in custom expr at level 1, *)
+(*         b1 custom expr at level 4, *)
+(*         b2 custom expr at level 4, *)
+(*         b3 custom expr at level 4, *)
+(*         bn custom expr at level 4, *)
+(*         ty constr at level 4). *)
 
 Notation "t1 t2" := (eApp t1 t2) (in custom expr at level 4, left associativity).
 Notation "( x )" := x (in custom expr, x at level 2).
 Notation "{ x }" := x (in custom expr, x constr).
 
 Module StdLib.
-
   Notation "a + b" := [| {eConst "Coq.Init.Nat.add"} {a} {b} |]
                         (in custom expr at level 0).
-  (* Notation "x" := x (in custom expr at level 0, x ident). *)
-  Notation "0" := [| {Z} |] ( in custom expr at level 0).
-  Notation "1" := [| {Suc} {Z} |] ( in custom expr at level 0).
+  Notation "'Z'" := (eConstr Nat_name "Z") ( in custom expr at level 0).
+  Notation "'Suc'" := (eConstr Nat_name "Suc") ( in custom expr at level 0).
+  Notation "0" := [| Z |] ( in custom expr at level 0).
+  Notation "1" := [| Suc Z |] ( in custom expr at level 0).
+
+  Notation "'Z'" := (pConstr "Z" [])
+                  (in custom pat at level 0).
+
+  Notation "'Suc' x" := (pConstr "Suc" [x])
+                    (in custom pat at level 0,
+                        x constr at level 4).
+
   Notation "'true'" := (pConstr "true" []) (in custom pat at level 0).
   Notation "'false'" := (pConstr "false" []) ( in custom pat at level 0).
 
-  Notation "'true'" := (eConstruct Bool_name 0) (in custom expr at level 0).
-  Notation "'false'" := (eConstruct Bool_name 1) ( in custom expr at level 0).
+  Notation "'true'" := (eConstr Bool_name "true") (in custom expr at level 0).
+  Notation "'false'" := (eConstr Bool_name "false") ( in custom expr at level 0).
+  (* Definition true := (pConstr "true" []). *)
+  (* Definition false := (pConstr "false" []). *)
+
+
+  Definition Σ : global_env :=
+    [gdInd Bool_name [("true", []); ("false", [])];
+     gdInd Nat_name  [("Z", []); ("Suc", [tyInd Nat_name])]].
 End StdLib.
 
 Import StdLib.
@@ -239,13 +327,14 @@ Check [| ^0 |].
 Check [| \x : Nat -> y |].
 
 Definition id_f_syn :=  [| (\x : Nat -> ^0) 1 |].
-Make Definition id_f_one := Eval compute in (expr_to_term id_f_syn).
+
+Make Definition id_f_one := Eval compute in (expr_to_term Σ id_f_syn).
 Example id_f_eq : id_f_one = 1. Proof. reflexivity. Qed.
 
 (* The same as [id_f_syn], but with named vars *)
 Definition id_f_with_vars := [| (\x : Nat -> x) 1 |].
 
-Make Definition id_f_one' := Eval compute in (expr_to_term (indexify [] id_f_with_vars)).
+Make Definition id_f_one' := Eval compute in (expr_to_term Σ (indexify [] id_f_with_vars)).
 Example id_f_eq' : id_f_one' = 1. Proof. reflexivity. Qed.
 
 Definition simple_let_syn :=
@@ -254,7 +343,7 @@ Definition simple_let_syn :=
      let y : Nat := 1 in ^0
    |].
 
-Make Definition simple_let := Eval compute in (expr_to_term simple_let_syn).
+Make Definition simple_let := Eval compute in (expr_to_term Σ simple_let_syn).
 Example simple_let_eq : simple_let 1 = 1. Proof. reflexivity. Qed.
 
 Definition simple_let_with_vars_syn :=
@@ -263,7 +352,7 @@ Definition simple_let_with_vars_syn :=
      let y : Nat := 1 in y
    |].
 
-Make Definition simple_let' := Eval compute in (expr_to_term (indexify [] simple_let_with_vars_syn)).
+Make Definition simple_let' := Eval compute in (expr_to_term Σ (indexify [] simple_let_with_vars_syn)).
 Example simple_let_eq' : simple_let' 0 = 1. Proof. reflexivity. Qed.
 
 
@@ -275,7 +364,7 @@ Definition negb_syn :=
           | false -> true
   |].
 
-Make Definition negb' := Eval compute in (expr_to_term (indexify [] negb_syn)).
+Make Definition negb' := Eval compute in (expr_to_term Σ (indexify [] negb_syn)).
 
 Example negb'_correct : forall b, negb' b = negb b.
 Proof.
@@ -285,4 +374,4 @@ Qed.
 Definition myplus_syn :=
   [| \x : Nat -> \y : Nat -> x + y |].
 
-Make Definition myplus := Eval compute in (expr_to_term (indexify [] myplus_syn)).
+Make Definition myplus := Eval compute in (expr_to_term Σ (indexify [] myplus_syn)).
