EvalE.v
@@ -18,8 +18,8 @@ Module Interpreter.
 
 
   Inductive val : Type :=
-  | vConstruct : inductive -> nat -> val
-  | vClos : env val -> name -> type -> expr -> val.
+  | vConstr : inductive -> name -> list val -> val
+  | vClos   : env val -> name -> type -> expr -> val.
 
   (* This doesn't work for the same reason as for STLC: in the case
      for application we don't know if [b] is decreasing.
@@ -38,15 +38,15 @@ Module Interpreter.
           | Some v' => Some v'
           | None => None
           end
-        | _, _ => None
+        | Some (vConstr ind n vs), Some v => Some (vConstr ind n (v :: vs))
+        | _,_ => None
         end
       | eConstruct t i =>
-        (* only nullary constructors *)
-        Some (vConstruct t i)
+        Some (vConstr t i [])
       | eConst nm => None
       | eCase (ind,i) ty e bs =>
         match (expr_eval ρ e) with
-        | Some (vConstruct ind' i) => if (string_dec ind ind') then
+        | Some (vConstr ind' i _) => if (string_dec ind ind') then
                                         match (List.nth_error bs i) with
                                         | Some v =>  expr_eval ρ (snd v)
                                         | _ => None
@@ -74,7 +74,25 @@ Module Interpreter.
 
   Definition todo := EvalError (A:=val) "Not implemented".
 
-  Fixpoint expr_eval (fuel : nat) (ρ : env val) (e : expr) : res val :=
+  Definition ind_name (v : val) :=
+    match v with
+    | vConstr ind_name _ _ => Some ind_name
+    | _ => None
+    end.
+
+  (* FIXME: should be extended to match the arguments of the constructor *)
+  Fixpoint match_pat (constr_name : name) (constr_args : list val) (bs : list (pat * expr)) :=
+    match bs with
+    | [] => None
+    | (p, e) :: bs' => if (andb (p.(pName) =? constr_name))
+                          (Nat.eqb (length constr_args) (length p.(pVars)))
+                     then
+                       let assignments := combine p.(pVars) constr_args in
+                       Some (assignments,e)
+                     else match_pat constr_name constr_args bs'
+    end.
+
+  Fixpoint expr_eval (fuel : nat) (Σ : global_env) (ρ : env val) (e : expr) : res val :=
     match fuel with
     | O => NotEnoughFuel
     | S n =>
@@ -85,25 +103,27 @@ Module Interpreter.
         Ok (vClos ρ nm ty b)
       | eLetIn nm e1 ty e2 => todo
       | eApp e1 e2 =>
-        match (expr_eval n ρ e1), (expr_eval n ρ e2) with
+        match (expr_eval n Σ ρ e1), (expr_eval n Σ ρ e2) with
         | Ok (vClos ρ' nm _ b), Ok v =>
-          match (expr_eval n (ρ' # [nm ~> v]) b) with
+          match (expr_eval n Σ (ρ' # [nm ~> v]) b) with
           | Ok v' => Ok v'
           | err => err
           end
-        | _, _ => EvalError "Error in App"
+        | Ok (vConstr ind n vs), Ok v => Ok (vConstr ind n (List.app vs [v]))
+        | EvalError msg, Ok _ => EvalError msg
+        | Ok _, EvalError msg => EvalError msg
+        | _,_ => EvalError "Error in App "
         end
-      | eConstruct t i =>
-        (* only nullary constructors *)
-        Ok (vConstruct t i)
+      | eConstr t i =>
+        Ok (vConstr t i [])
       | eConst nm => todo
       | eCase (ind,i) ty e bs =>
-        match (expr_eval n ρ e) with
-        | Ok (vConstruct ind' i) => if (string_dec ind ind') then
-                                        match (List.nth_error bs i) with
-                                        | Some v => expr_eval n ρ (snd v)
-                                        | _ => EvalError "No such constructor"
-                                        end
+        match (expr_eval n Σ ρ e) with
+        | Ok (vConstr ind' c vs) => if (string_dec ind ind') then
+                                      match (match_pat c vs bs) with
+                                      | Some (var_assign, v) => expr_eval n Σ (List.app ρ var_assign) v
+                                      | None => EvalError "No such constructor"
+                                      end
                                     else EvalError ("Expecting inductive " ++ ind ++
                                                      "but found " ++ ind')
         | _ => EvalError "Error in Case"
@@ -125,7 +145,7 @@ Module Interpreter.
      |].
 
   Example eval_prog1 :
-    expr_eval 3 [] prog1 = Ok (vConstruct "Coq.Init.Datatypes.bool" 1).
+    expr_eval 3 Σ [] prog1 = Ok (vConstr "Coq.Init.Datatypes.bool" "false" []).
   Proof. simpl. reflexivity. Qed.
 
 End Interpreter.
