Demo.v
@@ -27,12 +27,12 @@ Set Printing Notations.
 
 Import Interpreter.
 
-(* Execute the program using interpreter *)
-Compute (expr_eval 3 [] negb_app_true).
+(* Execute the program using the interpreter *)
+Compute (expr_eval 3 Σ [] negb_app_true).
 
 
 (* Make a Coq function from the AST of the program *)
-Make Definition coq_negb_app_true := Eval compute in (expr_to_term (indexify nil negb_app_true)).
+Make Definition coq_negb_app_true := Eval compute in (expr_to_term Σ (indexify nil negb_app_true)).
 
 Print coq_negb_app_true.
 
@@ -47,9 +47,9 @@ Definition my_negb :=
            | true -> false
            | false -> true) true  |].
 
-Compute (expr_eval 3 [] my_negb).
+Compute (expr_eval 3 Σ [] my_negb).
 
-Make Definition coq_my_negb := Eval compute in (expr_to_term (indexify [] my_negb)).
+Make Definition coq_my_negb := Eval compute in (expr_to_term Σ (indexify [] my_negb)).
 
 Fixpoint remove_by_key {A : Set} (key : string) (ρ : env A) : env A :=
     match ρ with
@@ -70,7 +70,7 @@ Fixpoint subst_env (ρ : env expr) (e : expr) : expr :=
   | eLambda nm ty b => eLambda nm ty (subst_env (remove_by_key nm ρ) b)
   | eLetIn nm e1 ty e2 => eLetIn nm (subst_env ρ e1) ty (subst_env (remove_by_key nm ρ) e2)
   | eApp e1 e2 => eApp (subst_env ρ e1) (subst_env ρ e2)
-  | eConstruct t i as e' => e'
+  | eConstr t i as e' => e'
   | eConst nm => eConst nm
   | eCase nm_i ty e bs =>
     (* TODO: this case is not complete! We ignore variables bound by patterns *)
@@ -79,9 +79,15 @@ Fixpoint subst_env (ρ : env expr) (e : expr) : expr :=
   end.
 
 
+Fixpoint vars_to_apps acc vs :=
+  match vs with
+  | [] => acc
+  | v :: vs' => vars_to_apps (eApp acc v) vs'
+  end.
+
 Fixpoint from_val (v : val) : expr :=
   match v with
-  | vConstruct x i => eConstruct x i
+  | vConstr x i vs => vars_to_apps (eConstr x i) (map from_val vs)
   | vClos ρ nm ty e => subst_env (map (fun x => (fst x, from_val (snd x))) ρ) (eLambda nm ty e)
   end.
 
@@ -89,10 +95,10 @@ Import MonadNotation.
 
 Run TemplateProgram
     (
-      t <- tmEval lazy (expr_eval 3 [] my_negb);;
+      t <- tmEval lazy (expr_eval 3 Σ [] my_negb);;
         match t with
           Ok v =>
-          t' <- tmEval lazy (expr_to_term (indexify [] (from_val v))) ;;
+          t' <- tmEval lazy (expr_to_term Σ (indexify [] (from_val v))) ;;
           def <- tmUnquoteTyped (bool -> bool) t' ;;
           tmDefinition "eval_my_negb" def ;;
              print_nf "Done."
@@ -106,3 +112,47 @@ Lemma my_negb_adequate : forall b, coq_my_negb b = eval_my_negb b.
 Proof.
   intros b; destruct b;auto.
 Qed.
+
+Definition is_zero_syn :=
+  [|
+
+      \x : Nat ->
+           case x : Nat_name return Bool of
+           | Z -> true
+           | Suc y -> false
+
+  |].
+
+Make Definition is_zero' := Eval compute in (expr_to_term Σ (indexify nil is_zero_syn)).
+
+
+Definition pred_syn :=
+  [|
+
+      \x : Nat ->
+           case x : Nat_name return Nat of
+           | Z -> x
+           | Suc y -> y
+
+  |].
+
+Make Definition pred' := Eval compute in (expr_to_term Σ (indexify nil pred_syn)).
+
+Definition prog2 := [| Suc (Suc Z) |].
+
+Compute (expr_eval 3 Σ [] prog2).
+
+Inductive blah :=
+  Bar : blah -> blah -> blah
+| Baz : blah.
+
+Definition Σ' : global_env :=
+  [gdInd "blah" [("Bar", [tyInd "blah"; tyInd "blah"]); ("Baz", [])];
+     gdInd Nat_name  [("Z", []); ("Suc", [tyInd Nat_name])]].
+
+Notation "'Bar'" := (eConstr "blah" "Bar") (in custom expr).
+Notation "'Baz'" := (eConstr "blah" "Baz") (in custom expr).
+
+Definition prog3 := [| Bar (Bar Baz Baz) Baz |].
+
+Compute (expr_eval 5 Σ [] prog3).
